reachability shortened proof

deps/poulet4/P4ABenchmarks/SmallFilterProof.v
@@ -6,183 +6,32 @@ From Hammer Require Import Tactics.
 Notation H := (IncrementalBits.header + BigBits.header).
 Notation A := IncrementalSeparate.aut.
 Notation conf := (P4automaton.configuration (P4A.interp A)).
+Definition r_states :=
+  Eval cbv in (Reachability.reachable_states IncrementalSeparate.aut 10 IncrementalBits.Start BigBits.Parse).
+
 Lemma prebisim_incremental_sep:
   pre_bisimulation IncrementalSeparate.aut
-                   (WPSymLeap.wp (H:=IncrementalSeparate.header))
-                   (reachable _ _ _ IncrementalSeparate.aut 10 IncrementalBits.Start BigBits.Parse)
+                   (WPSymLeap.wp r_states (H:=IncrementalSeparate.header))
+                   (Reachability.reachable_pair r_states)
                    nil
-                   (mk_init 10 IncrementalSeparate.aut IncrementalBits.Start BigBits.Parse)
+                   (mk_init _ _ _ IncrementalSeparate.aut 10 IncrementalBits.Start BigBits.Parse)
                    (inl (inl IncrementalBits.Start), [], [])
                    (inl (inr BigBits.Parse), [], []).
 Proof.
-  set (r := (mk_init 10 IncrementalSeparate.aut IncrementalBits.Start BigBits.Parse)).
+  set (r := (mk_init _ _ _ IncrementalSeparate.aut 10 IncrementalBits.Start BigBits.Parse)).
   cbv in r.
   subst r.
-  match goal with
-  | |- pre_bisimulation ?a ?wp ?i ?R (?C :: _) _ _ =>
-    let H := fresh "H" in
-    assert
-      (H :
-         ~
-           (forall q1 q2 : P4automaton.configuration (P4A.interp a),
-               interp_crel i R q1 q2 -> interp_conf_rel C q1 q2))
-  end.
-  
-  set (a:=IncrementalSeparate.aut).
-  set (i:=(reachable IncrementalBits.state BigBits.state
-        (Sum.H IncrementalBits.header BigBits.header) A 10 IncrementalBits.Start
-        BigBits.Parse)) in *.
-  rewrite (filter_entails (a:=a)) by typeclasses eauto.
-  simpl.
-  rewrite (no_state) by typeclasses eauto.
-  repeat
-    unfold interp_conf_rel, interp_conf_state, interp_state_template, interp_store_rel
-     || cbn; eapply forall_exists; repeat (setoid_rewrite  <- split_univ; cbn).
-  repeat (setoid_rewrite  <- split_ex; cbn).
-  unfold not.
-  eexists.
-  eexists.
-  exact tt.
-  intros.
-  eapply H.
-  exact tt.
+  solve_bisim.
+  solve_bisim.
+  solve_bisim.
+  solve_bisim.
+  solve_bisim.
+  solve_bisim.
+  solve_bisim.
   cbv.
-
-  break_store.
   sauto.
-  solve [ sauto | unfold not; now break_store ].
-
-
-  ; pose (t := wp a C);
-    eapply PreBisimulationExtend with (H0 := right H) (W := t);
-      [ tauto | reflexivity |  ]; compute in t; simpl (_ ++ _); 
-        unfold t; clear t; clear H
-  end.
-  
-         | |- pre_bisimulation ?a ?wp ?i ?R (?C :: _) _ _ =>
-           skip_bisim a wp i R C;
-             idtac "Entailment holds:";
-             let g := constr:(forall q1 q2 : P4automaton.configuration (P4A.interp a),
-                          interp_crel i R q1 q2 -> interp_conf_rel C q1 q2) in
-             idtac g
-         | |- pre_bisimulation _ _ _ _ [] _ _ => apply PreBisimulationClose
-         end.
-  (*time (repeat (solve_bisim)).*)
-  repeat (unfold interp_conf_rel, interp_conf_state, interp_state_template || cbn).
-  intuition eauto;
-  firstorder (try congruence);
-  sauto limit:5000.
-
   Unshelve.
-  all: (exact nil).
-  
-Time Qed.
-
-Ltac break_store2 h0 h1 := 
-  repeat match goal with
-  | |- exists (x: P4A.store ?H), @?P x =>
-    cut (exists y0 y1,
-                P ([(h0, P4A.VBits y0);
-                    (h1, P4A.VBits y1)]));
-    [ intros [x0 [x1 ?]];
-      exists ([(h0, P4A.VBits x0);
-          (h1, P4A.VBits x1)]);
-      eauto
-      | trivial
-    ];
-    repeat eexists
-  | |- (forall (x: P4A.store ?H), _) -> False =>
-      intros
-  | H: forall (x: P4A.store ?H), @?P x |- _ =>
-      assert (forall y0 y1,
-                  P ([(h0, P4A.VBits y0);
-                      (h1, P4A.VBits y1)])); [
-      cbn; sauto | 
-      sauto
-    ]
-  end.
-
-Ltac break_store4 h0 h1 h2 h3 := 
-  repeat match goal with
-  | |- exists (x: P4A.store ?H), @?P x =>
-    cut (exists y0 y1 y2 y3,
-                P ([(h0, P4A.VBits y0);
-                    (h1, P4A.VBits y1);
-                    (h2, P4A.VBits y2);
-                    (h3, P4A.VBits y3)]));
-    [ intros [x0 [x1 [x2 [x3 ?]]]];
-      exists ([(h0, P4A.VBits x0);
-          (h1, P4A.VBits x1);
-          (h2, P4A.VBits x2);
-          (h3, P4A.VBits x3)]);
-      eauto
-      | trivial
-    ];
-    repeat eexists
-  | |- (forall (x: P4A.store ?H), _) -> False =>
-      intros
-  | H: forall (x: P4A.store ?H), @?P x |- _ =>
-      assert (forall y0 y1 y2 y3,
-                  P ([(h0, P4A.VBits y0);
-                      (h1, P4A.VBits y1);
-                      (h2, P4A.VBits y2);
-                      (h3, P4A.VBits y3)])); [
-      cbn; sauto | 
-      match goal with |- ?H => idtac H end
-    ]
-  end.
-
-Ltac break_store :=
-  match goal with
-  | |- context[ P4A.store ?H ] =>
-    let hs := fresh "hdrs" in
-    pose (hs := FinType.enum H);
-    cbv in hs;
-    match find hs with
-    | [?h0; ?h1] => break_store2 h0 h1
-    | [?h0; ?h1; ?h2; ?h3] => break_store4 h0 h1 h2 h3
-    | _ => idtac hs
-    end
-  end.
-
-
-Lemma intermediate_example:
-  ~ (forall q1 q2 : conf,
- interp_crel
-   (separated IncrementalBits.state BigBits.state
-      (Sum.H IncrementalBits.header BigBits.header) A)
-   [(BCSnoc BCEmp 1), ⟨ inl (inl IncrementalBits.Start), 0 ⟩ ⟨ 
-    inl (inr BigBits.Parse), 1
-    ⟩ ⊢ (BREq (BEHdr (BCSnoc BCEmp 1) Left (Syntax.HRVar (inl IncrementalBits.Pref)))
-           (BELit (IncrementalBits.header + BigBits.header) (BCSnoc BCEmp 1) [true])
-         ⇒ (BREq (BEHdr (BCSnoc BCEmp 1) Right (Syntax.HRVar (inr BigBits.Pref)))
-              (BELit (IncrementalBits.header + BigBits.header) (BCSnoc BCEmp 1) [true])
-            ⇒ bfalse));
-   BCEmp, ⟨ inl (inl IncrementalBits.Finish), 0 ⟩ ⟨ inr true, 0 ⟩ ⊢ bfalse] q1 q2 ->
- interp_conf_rel (BCEmp, ⟨ inr true, 0 ⟩ ⟨ inl (inr BigBits.Parse), 1 ⟩ ⊢ bfalse) q1 q2).
-Proof.
-  rewrite (no_state _).
-  repeat (unfold interp_conf_rel, interp_conf_state, interp_state_template, interp_store_rel || cbn).
-  eapply forall_exists.
-  repeat (setoid_rewrite <- split_univ; cbn).
-  repeat (setoid_rewrite <- split_ex; cbn).
-  unfold not.
-  Print break_store.
-  break_store.
-
-  intros [[st1 store1] buf1] [[st2 store2] buf2].
-  unfold interp_crel, interp_conf_rel, interp_conf_rel, interp_conf_state, interp_state_template; cbn.
-  simpl;
-  rewrite (no_state i) by (typeclasses eauto);
-  repeat (unfold interp_conf_rel, interp_conf_state, interp_state_template, interp_store_rel || cbn);
-  eapply forall_exists;
-  repeat (setoid_rewrite <- split_univ; cbn);
-  repeat (setoid_rewrite <- split_ex; cbn);
-  (solve [sauto | unfold not; now break_store]).
-
-  intros.
-  intuition.
-  break_store.
-  break_store2
-  break_store4 BigBits.Pref BigBits.Suf IncrementalBits.Pref IncrementalBits.Suf.
-  cbv.
+  exact nil.
+  exact nil.
+  exact nil.
+Qed.
